add post-conditions in Lib.PQ.Buffer

lib/fst/Lib.PQ.Buffer.fst
@@ -2,106 +2,122 @@ module Lib.PQ.Buffer
 
 open FStar.HyperStack
 open FStar.HyperStack.ST
+
 open LowStar.ModifiesPat
 open LowStar.Modifies
-
-module Buf = LowStar.Buffer
-module U32 = FStar.UInt32
-module ST = FStar.HyperStack.ST
-module HS = FStar.HyperStack
-
-//module Seq = FStar.Seq
-module Seq = Lib.Sequence
 
 open Lib.IntTypes
 open Lib.RawIntTypes
 
+module B = LowStar.Buffer
+module U32 = FStar.UInt32
+module ST = FStar.HyperStack.ST
+module HS = FStar.HyperStack
+
+module Seq = Lib.Sequence
+module ByteSeq = Lib.ByteSequence
+
 unfold let v = size_v
 
-type lbuffer (a:Type0) (len:size_nat) = b:Buf.buffer a {Buf.length b == len}
+type lbuffer (a:Type0) (len:size_nat) = b:B.buffer a {B.length b == len}
 
 inline_for_extraction
 val sub:
-  #a:Type0 -> #len:size_nat -> #olen:size_nat ->
-  b:lbuffer a len -> start:size_t ->
-  n:size_t{v start + v n <= len /\ v n == olen} -> Stack (lbuffer a olen)
-  (requires (fun h0 -> Buf.live h0 b))
-  (ensures (fun h0 r h1 -> h0 == h1 /\ r == Buf.gsub b (size_to_UInt32 start) (size_to_UInt32 n)))
+    #a:Type0
+  -> #len:size_nat
+  -> #olen:size_nat
+  -> b:lbuffer a len
+  -> start:size_t
+  -> n:size_t{v start + v n <= len /\ v n == olen}
+  -> Stack (lbuffer a olen)
+    (requires fun h0 -> B.live h0 b)
+    (ensures  fun h0 r h1 -> h0 == h1 /\ r == B.gsub b (size_to_UInt32 start) (size_to_UInt32 n))
 let sub #a #len #olen b start n =
-  Buf.sub b (size_to_UInt32 start) (size_to_UInt32 n)
+  B.sub b (size_to_UInt32 start) (size_to_UInt32 n)
 
 inline_for_extraction
 val index:
-  #a:Type0 -> #len:size_nat ->
-  b:lbuffer a len -> i:size_t{v i < len} -> Stack a
-  (requires (fun h0 -> Buf.live h0 b))
-  (ensures (fun h0 r h1 -> h0 == h1 /\ r == Seq.index #a #len (Buf.as_seq h1 b) (v i)))
+    #a:Type0
+  -> #len:size_nat
+  -> b:lbuffer a len
+  -> i:size_t{v i < len}
+  -> Stack a
+    (requires fun h0 -> B.live h0 b)
+    (ensures  fun h0 r h1 -> h0 == h1 /\ r == Seq.index #a #len (B.as_seq h1 b) (v i))
 let index #a #len b i =
-  Buf.index b (size_to_UInt32 i)
+  B.index b (size_to_UInt32 i)
 
 inline_for_extraction
 val upd:
-  #a:Type0 -> #len:size_nat{len > 0} ->
-  b:lbuffer a len -> i:size_t{v i < len} ->
-  x:a -> Stack unit
-  (requires (fun h0 -> Buf.live h0 b))
-  (ensures (fun h0 _ h1 ->
-    Buf.modifies_1 b h0 h1 /\ Buf.live h1 b /\
-    Buf.as_seq h1 b == Seq.upd #a #len (Buf.as_seq h0 b) (v i) x))
+    #a:Type0
+  -> #len:size_nat{len > 0}
+  -> b:lbuffer a len
+  -> i:size_t{v i < len}
+  -> x:a
+  -> Stack unit
+    (requires fun h0 -> B.live h0 b)
+    (ensures  fun h0 _ h1 ->
+      B.modifies_1 b h0 h1 /\ B.live h1 b /\
+      B.as_seq h1 b == Seq.upd #a #len (B.as_seq h0 b) (v i) x)
 let upd #a #len b i v =
-  Buf.upd b (size_to_UInt32 i) v
+  B.upd b (size_to_UInt32 i) v
 
 inline_for_extraction let op_Array_Assignment #a #len = upd #a #len
 inline_for_extraction let op_Array_Access #a #len = index #a #len
 
 inline_for_extraction
 val create:
-  #a:Type0 -> #len:size_nat{len > 0} ->
-  clen:size_t{v clen == len} -> init:a -> StackInline (lbuffer a len)
-  (requires (fun h0 -> True))
-  (ensures (fun h0 r h1 ->
-    Buf.alloc_post_common (HS.get_tip h0) len r h0 h1 /\
-    Buf.as_seq h1 r == Seq.create len init))
+    #a:Type0
+  -> #len:size_nat{len > 0}
+  -> clen:size_t{v clen == len}
+  -> init:a
+  -> StackInline (lbuffer a len)
+    (requires fun h0 -> True)
+    (ensures  fun h0 r h1 ->
+      B.alloc_post_common (HS.get_tip h0) len r h0 h1 /\
+      B.as_seq h1 r == Seq.create len init)
 let create #a #len clen init =
-  Buf.alloca init (size_to_UInt32 clen)
+  B.alloca init (size_to_UInt32 clen)
 
 inline_for_extraction
 val createL:
-  #a:Type0 -> init:list a{List.Tot.length init <= max_size_t} ->
-  StackInline (lbuffer a (List.Tot.length init))
-  (requires (fun h0 -> Buf.alloc_of_list_pre #a init))
-  (ensures (fun h0 r h1 ->
-    let len = FStar.List.Tot.length init in
-    Buf.alloc_post_common (HS.get_tip h0) len r h0 h1 /\
-    Buf.as_seq h1 r == Seq.of_list init /\
-    Buf.alloc_of_list_post #a len r))
+    #a:Type0
+  -> init:list a{List.Tot.length init <= max_size_t}
+  -> StackInline (lbuffer a (List.Tot.length init))
+    (requires fun h0 -> B.alloc_of_list_pre #a init)
+    (ensures fun h0 r h1 ->
+      let len = FStar.List.Tot.length init in
+      B.alloc_post_common (HS.get_tip h0) len r h0 h1 /\
+      B.as_seq h1 r == Seq.of_list init /\
+      B.alloc_of_list_post #a len r)
 let createL #a init =
-  Buf.alloca_of_list init
+  B.alloca_of_list init
 
 inline_for_extraction
-val recall
-  (#a:Type)
-  (#len:size_nat)
-  (b:lbuffer a len)
-: Stack unit
-  (requires (fun _ -> Buf.recallable b))
-  (ensures  (fun m0 _ m1 -> m0 == m1 /\ Buf.live m1 b))
-let recall #a #len b = Buf.recall b
+val recall:
+  #a:Type
+  -> #len:size_nat
+  -> b:lbuffer a len
+  -> Stack unit
+  (requires fun _ -> B.recallable b)
+  (ensures  fun m0 _ m1 -> m0 == m1 /\ B.live m1 b)
+let recall #a #len b = B.recall b
 
 inline_for_extraction
 val createL_global:
-  #a:Type0 -> init:list a{List.Tot.length init <= max_size_t} ->
-  ST (lbuffer a (List.Tot.length init))
-  (requires fun h0 -> Buf.alloc_of_list_pre #a init)
-  (ensures  fun h0 b h1 ->
-    let len = FStar.List.Tot.length init in
-    Buf.recallable b /\
-    Buf.alloc_post_static HyperStack.root len b /\
-    Buf.alloc_of_list_post len b /\
-    Buf.alloc_post_common HyperStack.root len b h0 h1 /\
-    Buf.as_seq h1 b == Seq.of_list init)
+    #a:Type0
+  -> init:list a{List.Tot.length init <= max_size_t}
+  -> ST (lbuffer a (List.Tot.length init))
+    (requires fun h0 -> B.alloc_of_list_pre #a init)
+    (ensures  fun h0 b h1 ->
+      let len = FStar.List.Tot.length init in
+      B.recallable b /\
+      B.alloc_post_static HyperStack.root len b /\
+      B.alloc_of_list_post len b /\
+      B.alloc_post_common HyperStack.root len b h0 h1 /\
+      B.as_seq h1 b == Seq.of_list init)
 let createL_global #a init =
-  Buf.gcmalloc_of_list HyperStack.root init
+  B.gcmalloc_of_list HyperStack.root init
 
 
 // val lemma_seq_slice_index:
@@ -119,16 +135,16 @@ let createL_global #a init =
 //   #a:Type -> #len:size_nat ->
 //   o:lbuffer a len -> clen:size_t{v clen == len} ->
 //   i:lbuffer a len -> Stack unit
-//   (requires (fun h0 -> Buf.live h0 o /\ Buf.live h0 i /\ Buf.disjoint i o))
+//   (requires (fun h0 -> B.live h0 o /\ B.live h0 i /\ B.disjoint i o))
 //   (ensures (fun h0 _ h1 ->
-//     Buf.live h1 o /\ Buf.live h1 i /\ modifies (loc_buffer o) h0 h1 /\
-//     Buf.as_seq h1 o == Buf.as_seq h0 i))
+//     B.live h1 o /\ B.live h1 i /\ modifies (loc_buffer o) h0 h1 /\
+//     B.as_seq h1 o == B.as_seq h0 i))
 // let copy #a #len o clen i =
 //   let h0 = ST.get() in
 //   let inv (h1:mem) (j:nat{j <= len}) =
-//     Buf.live h1 o /\ Buf.live h1 i /\
+//     B.live h1 o /\ B.live h1 i /\
 //     modifies (loc_buffer o) h0 h1 /\
-//     Seq.slice (Buf.as_seq h1 o) 0 j == Seq.slice (Buf.as_seq h0 i) 0 j in
+//     Seq.slice (B.as_seq h1 o) 0 j == Seq.slice (B.as_seq h0 i) 0 j in
 //   let f' (j:size_t{0 <= v j /\ v j < len}) : Stack unit
 //       (requires (fun h -> inv h (v j)))
 //       (ensures (fun h1 _ h2 -> inv h2 (v j + 1))) =
@@ -136,56 +152,106 @@ let createL_global #a init =
 //       let src_i = i.(j) in
 //       o.(j) <- src_i;
 //       let h2 = ST.get () in
-//       lemma_seq_slice_index (Buf.as_seq h2 o) (Buf.as_seq h0 i) (v j);
+//       lemma_seq_slice_index (B.as_seq h2 o) (B.as_seq h0 i) (v j);
 //       modifies_trans (loc_buffer o) h0 h1 (loc_buffer o) h2 in
 //   Lib.Loops.for (size 0) clen inv f'
 
 inline_for_extraction
 val copy:
-  #a:Type -> #len:size_nat ->
-  o:lbuffer a len -> clen:size_t{v clen == len} ->
-  i:lbuffer a len -> Stack unit
-  (requires (fun h0 -> Buf.live h0 o /\ Buf.live h0 i /\ Buf.disjoint i o))
-  (ensures (fun h0 _ h1 ->
-    Buf.live h1 o /\ Buf.live h1 i /\ modifies (loc_buffer o) h0 h1 /\
-    Buf.as_seq h1 o == Buf.as_seq h0 i))
+    #a:Type
+  -> #len:size_nat
+  -> o:lbuffer a len
+  -> clen:size_t{v clen == len}
+  -> i:lbuffer a len
+  -> Stack unit
+    (requires fun h0 -> B.live h0 o /\ B.live h0 i /\ B.disjoint i o)
+    (ensures  fun h0 _ h1 ->
+      B.live h1 o /\ B.live h1 i /\ modifies (loc_buffer o) h0 h1 /\
+      B.as_seq h1 o == B.as_seq h0 i)
 let copy #a #len o clen i =
   let h0 = ST.get () in
   LowStar.BufferOps.blit i (size_to_UInt32 (size 0)) o (size_to_UInt32 (size 0)) (size_to_UInt32 clen);
   let h1 = ST.get () in
-  assert (Seq.slice #a #len (Buf.as_seq h1 o) 0 len == Seq.slice #a #len (Buf.as_seq h0 i) 0 len)
+  assert (Seq.slice #a #len (B.as_seq h1 o) 0 len == Seq.slice #a #len (B.as_seq h0 i) 0 len)
 
-let loop_nospec_inv (#a:Type) (h0:mem) (h1:mem)
-		    (len:size_nat) (n:size_nat)
-		    (buf:lbuffer a len) (i:size_nat{i <= n}): Type =
-   Buf.live h0 buf /\ Buf.live h1 buf /\ modifies (loc_buffer buf) h0 h1
+inline_for_extraction
+val update_sub:
+    #a:Type
+  -> #len:size_nat
+  -> dst:lbuffer a len
+  -> start:size_t{v start < len}
+  -> n:size_t{v start + v n <= len}
+  -> src:lbuffer a (v n)
+  -> Stack unit
+    (requires fun h -> B.live h dst /\ B.live h src /\ B.disjoint dst src)
+    (ensures  fun h0 _ h1 -> B.live h1 dst /\ modifies (loc_buffer dst) h0 h1 /\
+      B.as_seq h1 dst == Seq.update_sub #a #len (B.as_seq h0 dst) (v start) (v n) (B.as_seq h0 src))
+let update_sub #a #len dst start n src =
+  let h0 = ST.get () in
+  let b = sub dst start n in
+  copy b n src;
+  let h1 = ST.get () in
+
+  assert (B.as_seq h1 b == B.as_seq h0 src);
+  assert (forall (k:size_nat{0 <= k /\ k < v n}). Seq.index #_ #(v n) (B.as_seq h1 b) k == Seq.index #_ #(v n) (B.as_seq h0 src) k);
+  assert (forall (k:size_nat{0 <= k /\ k < v start /\ v start + v n <= k /\ k < len}). Seq.index #_ #len (B.as_seq h1 dst) k == Seq.index #_ #len (B.as_seq h0 dst) k);
+
+  assert (forall (k:size_nat{0 <= k /\ k < v start /\ v start + v n <= k /\ k < len}). Seq.index #_ #len (B.as_seq h1 dst) k ==
+    Seq.index (Seq.update_sub #a #len (B.as_seq h0 dst) (v start) (v n) (B.as_seq h0 src)) k);
+  assert (forall (k:size_nat{v start <= k /\ k < v start + v n}). Seq.index #_ #len (B.as_seq h1 dst) k ==
+    Seq.index (Seq.update_sub #a #len (B.as_seq h0 dst) (v start) (v n) (B.as_seq h0 src)) k);
+
+  assume (forall (k:size_nat{0 <= k /\ k < len}). Seq.index #_ #len (B.as_seq h1 dst) k ==
+    Seq.index (Seq.update_sub #a #len (B.as_seq h0 dst) (v start) (v n) (B.as_seq h0 src)) k); //FIXME
+
+  Seq.eq_intro (B.as_seq h1 dst) (Seq.update_sub #a #len (B.as_seq h0 dst) (v start) (v n) (B.as_seq h0 src))
+
+inline_for_extraction noextract private
+val loop_nospec_inv:
+    #a:Type
+  -> h0:mem
+  -> h1:mem
+  -> len:size_nat
+  -> n:size_nat
+  -> buf:lbuffer a len
+  -> i:size_nat{i <= n}
+  -> Type0
+let loop_nospec_inv #a h0 h1 len n buf i =
+  B.live h0 buf /\ B.live h1 buf /\ modifies (loc_buffer buf) h0 h1
 
 inline_for_extraction
 val loop_nospec:
-  #h0:mem -> #a:Type0 -> #len:size_nat ->
-  n:size_t -> buf:lbuffer a len ->
-  impl:
-    (i:size_t{v i < v n} -> Stack unit
-      (requires fun h -> loop_nospec_inv #a h0 h len (v n) buf (v i))
-      (ensures  fun _ r h1 -> loop_nospec_inv #a h0 h1 len (v n) buf (v i + 1))) -> Stack unit
-  (requires (fun h -> h0 == h /\ Buf.live h0 buf))
-  (ensures (fun _ _ h1 -> Buf.live h1 buf /\ modifies (loc_buffer buf) h0 h1))
+    #h0:mem
+  -> #a:Type0
+  -> #len:size_nat
+  -> n:size_t
+  -> buf:lbuffer a len
+  -> impl:
+      (i:size_t{v i < v n} -> Stack unit
+        (requires fun h -> loop_nospec_inv #a h0 h len (v n) buf (v i))
+        (ensures  fun _ r h1 -> loop_nospec_inv #a h0 h1 len (v n) buf (v i + 1)))
+  -> Stack unit
+    (requires fun h -> h0 == h /\ B.live h0 buf)
+    (ensures  fun _ _ h1 -> B.live h1 buf /\ modifies (loc_buffer buf) h0 h1)
 let loop_nospec #h0 #a #len n buf impl =
-  let inv (h1:mem) (j:nat{j <= v n}) =
+  let inv h1 (j:nat{j <= v n}) =
     loop_nospec_inv #a h0 h1 len (v n) buf j in
   let f' (j:size_t{0 <= v j /\ v j < v n}): Stack unit
-      (requires (fun h -> inv h (v j)))
-      (ensures (fun _ _ h2 -> inv h2 (v j + 1))) =
+      (requires fun h -> inv h (v j))
+      (ensures  fun _ _ h2 -> inv h2 (v j + 1)) =
       impl j in
   Lib.Loops.for (size 0) n inv f'
 
+
 inline_for_extraction
 val uint_from_bytes_le:
-  #t:m_inttype{~(SIZE? t)} ->
-  i:lbuffer uint8 (numbytes t) ->
-  Stack (uint_t t)
-  (requires (fun h0 -> Buf.live h0 i))
-  (ensures (fun h0 o h1 -> h0 == h1 /\ Buf.live h1 i))
+    #t:m_inttype{~(SIZE? t)}
+  -> i:lbuffer uint8 (numbytes t)
+  -> Stack (uint_t t)
+    (requires fun h0 -> B.live h0 i)
+    (ensures  fun h0 o h1 ->
+      h0 == h1 /\ B.live h1 i /\
+      o == ByteSeq.uint_from_bytes_le #t (B.as_seq h0 i))
 let uint_from_bytes_le #t i =
   match t with
   | U8 -> i.(size 0)
@@ -196,10 +262,13 @@ let uint_from_bytes_le #t i =
 
 inline_for_extraction
 val uint_from_bytes_be:
-  #t:m_inttype{~(SIZE? t)} ->
-  i:lbuffer uint8 (numbytes t) -> Stack (uint_t t)
-  (requires (fun h0 -> Buf.live h0 i))
-  (ensures (fun h0 o h1 -> h0 == h1 /\ Buf.live h1 i))
+    #t:m_inttype{~(SIZE? t)}
+  -> i:lbuffer uint8 (numbytes t)
+  -> Stack (uint_t t)
+    (requires fun h0 -> B.live h0 i)
+    (ensures  fun h0 o h1 ->
+      h0 == h1 /\ B.live h1 i /\
+      o == ByteSeq.uint_from_bytes_be #t (B.as_seq h0 i))
 let uint_from_bytes_be #t i =
   match t with
   | U8 -> i.(size 0)
@@ -210,11 +279,14 @@ let uint_from_bytes_be #t i =
 
 inline_for_extraction
 val uint_to_bytes_le:
-  #t:m_inttype{~(SIZE? t)} ->
-  o:lbuffer uint8 (numbytes t) ->
-  i:uint_t t -> Stack unit
-  (requires (fun h0 -> Buf.live h0 o))
-  (ensures (fun h0 _ h1 -> Buf.live h1 o /\ modifies (loc_buffer o) h0 h1))
+    #t:m_inttype{~(SIZE? t)}
+  -> o:lbuffer uint8 (numbytes t)
+  -> i:uint_t t
+  -> Stack unit
+    (requires fun h0 -> B.live h0 o)
+    (ensures  fun h0 _ h1 ->
+      B.live h1 o /\ modifies (loc_buffer o) h0 h1 /\
+      B.as_seq h1 o == ByteSeq.uint_to_bytes_le #t i)
 let uint_to_bytes_le #t o i =
   match t with
   | U8 -> o.(size 0) <- i
@@ -225,11 +297,14 @@ let uint_to_bytes_le #t o i =
 
 inline_for_extraction
 val uint_to_bytes_be:
-  #t:m_inttype{~(SIZE? t)} ->
-  o:lbuffer uint8 (numbytes t) ->
-  i:uint_t t -> Stack unit
-  (requires (fun h0 -> Buf.live h0 o))
-  (ensures (fun h0 _ h1 -> Buf.live h1 o /\ modifies (loc_buffer o) h0 h1))
+    #t:m_inttype{~(SIZE? t)}
+  -> o:lbuffer uint8 (numbytes t)
+  -> i:uint_t t
+  -> Stack unit
+    (requires fun h0 -> B.live h0 o)
+    (ensures  fun h0 _ h1 ->
+      B.live h1 o /\ modifies (loc_buffer o) h0 h1 /\
+      B.as_seq h1 o == ByteSeq.uint_to_bytes_be #t i)
 let uint_to_bytes_be #t o i =
   match t with
   | U8 -> o.(size 0) <- i
@@ -239,5 +314,9 @@ let uint_to_bytes_be #t o i =
   | U128 -> C.store128_be o (u128_to_UInt128 i)
 
 assume val print_compare_display:
-  len:size_t -> lbuffer uint8 (size_v len) ->
-  lbuffer uint8 (size_v len) -> Stack unit (requires (fun h -> True)) (ensures (fun h0 _ h1 -> True))
+    len:size_t
+  -> lbuffer uint8 (size_v len)
+  -> lbuffer uint8 (size_v len)
+  -> Stack unit
+    (requires fun h -> True)
+    (ensures fun h0 _ h1 -> True)
